permissions in Steel.ST.Array

pulse/ulib/experimental/Steel.ST.Array.fst
@@ -40,35 +40,36 @@ let repr (#t:_) (r:array t) = FStar.Seq.lseq t (length r)
 /// The main representation predicate
 let pts_to (#t:Type)
            (a:array t)
+           (p:perm)
            ([@@@smt_fallback]x:seq t)
   : vprop
   = exists_ (fun (r:repr a) ->
       pure (eq2 #(seq t) r x) `star`
-      A.varray_pts_to a r)
+      A.varray_pts_to a p r)
 
-let intro_pts_to #t #o (a:array t) (s:repr a) (s':seq t)
+let intro_pts_to #t #o #p (a:array t) (s:repr a) (s':seq t)
   : STGhost unit o
-      (A.varray_pts_to a s)
-      (fun _ -> pts_to a s')
+      (A.varray_pts_to a p s)
+      (fun _ -> pts_to a p s')
       (requires s == s')
       (ensures fun _ -> True)
   = intro_pure (s == s');
-    intro_exists s (fun (s:repr a) -> pure (s == s') `star` A.varray_pts_to a s)
+    intro_exists s (fun (s:repr a) -> pure (s == s') `star` A.varray_pts_to a p s)
 
-let elim_pts_to #t #o (a:array t) (s:seq t)
+let elim_pts_to #t #o #p (a:array t) (s:seq t)
   : STGhost (erased (repr a)) o
-      (pts_to a s)
-      (fun s' -> A.varray_pts_to a s')
+      (pts_to a p s)
+      (fun s' -> A.varray_pts_to a p s')
       (requires True)
       (ensures fun s' -> eq2 #(seq t) s' s)
   = let s = elim_exists () in
     elim_pure _;
     s
 
-let pts_to_length #t #o (a:array t) (s:seq t)
+let pts_to_length #t #o #p (a:array t) (s:seq t)
   : STGhost unit o
-      (pts_to a s)
-      (fun _ -> pts_to a s)
+      (pts_to a p s)
+      (fun _ -> pts_to a p s)
       (requires True)
       (ensures fun _ -> Seq.length s == length a)
   = let s' = elim_pts_to a s in
@@ -79,7 +80,7 @@ let alloc_pt (#t:Type)
              (n:U32.t)
   : SE.SteelT (larray t (U32.v n))
            emp
-           (fun r -> pts_to r (Seq.create (U32.v n) x))
+           (fun r -> pts_to r full_perm (Seq.create (U32.v n) x))
   = let a = A.malloc x n in
     let s = A.intro_varray_pts_to a in
     intro_pts_to a s (Seq.create (U32.v n) x);
@@ -90,16 +91,17 @@ let alloc (#t:Type)
           (n:U32.t)
   : STT (larray t (U32.v n))
         emp
-        (fun r -> pts_to r (Seq.create (U32.v n) x))
+        (fun r -> pts_to r full_perm (Seq.create (U32.v n) x))
   = let x = coerce_steel (fun _ -> alloc_pt x n) in x
 
 let read_pt (#t:Type)
-              (a:array t)
-              (#s:erased (seq t))
-               (i:U32.t { U32.v i < Seq.length s })
+            (#p:perm)
+            (a:array t)
+            (#s:erased (seq t))
+            (i:U32.t { U32.v i < Seq.length s })
   : SE.Steel t
-       (pts_to a s)
-       (fun _ -> pts_to a s)
+       (pts_to a p s)
+       (fun _ -> pts_to a p s)
        (requires fun _ -> True)
        (ensures fun _ v _ ->
          v == Seq.index s (U32.v i))
@@ -108,18 +110,19 @@ let read_pt (#t:Type)
     let x = A.index a i in
     let _ = A.intro_varray_pts_to a in
     SEA.change_equal_slprop
-              (A.varray_pts_to _ _)
-              (A.varray_pts_to _ _);
+              (A.varray_pts_to _ _ _)
+              (A.varray_pts_to _ _ _);
     intro_pts_to a s' s;
     return x
 
 let read (#t:Type)
+         (#p:perm)
          (a:array t)
          (#s:erased (seq t))
          (i:U32.t { U32.v i < Seq.length s })
   : ST t
-       (pts_to a s)
-       (fun _ -> pts_to a s)
+       (pts_to a p s)
+       (fun _ -> pts_to a p s)
        (requires True)
        (ensures fun v ->
          v == Seq.index s (U32.v i))
@@ -131,8 +134,8 @@ let write_pt (#t:Type)
              (i:U32.t { U32.v i < Seq.length s })
              (x:t)
   : SE.SteelT unit
-       (pts_to a s)
-       (fun _ -> pts_to a (Seq.upd s (U32.v i) x))
+       (pts_to a full_perm s)
+       (fun _ -> pts_to a full_perm (Seq.upd s (U32.v i) x))
   = let s' = elim_pts_to a s in
     A.elim_varray_pts_to a s';
     A.upd a i x;
@@ -146,13 +149,13 @@ let write (#t:Type)
           (i:U32.t { U32.v i < Seq.length s })
           (x:t)
   : STT unit
-       (pts_to a s)
-       (fun _ -> pts_to a (Seq.upd s (U32.v i) x))
+       (pts_to a full_perm s)
+       (fun _ -> pts_to a full_perm (Seq.upd s (U32.v i) x))
   = coerce_steel (fun _ -> write_pt a i x); ()
 
 let free_pt (#t:Type) (a:array t) (#s:erased (repr a))
   : SE.SteelT unit
-       (A.varray_pts_to a s)
+       (A.varray_pts_to a full_perm s)
        (fun _ -> emp)
   = A.elim_varray_pts_to a s;
     A.free a;
@@ -160,19 +163,20 @@ let free_pt (#t:Type) (a:array t) (#s:erased (repr a))
 
 let free (#t:Type) (a:array t)
   : STT unit
-       (exists_ (pts_to a))
+       (exists_ (pts_to a full_perm))
        (fun _ -> emp)
   = let _ = elim_exists () in
     let s = elim_pts_to a _ in
     coerce_steel (fun _ -> free_pt a #s)
 
 let memcpy_pt (#t:_)
+              (#p0:perm)
               (a0 a1:array t)
               (#s0 #s1:erased (seq t))
               (l:U32.t { U32.v l == length a0 /\ length a0 == length a1 } )
   : SE.SteelT unit
-      (pts_to a0 s0 `star` pts_to a1 s1)
-      (fun _ -> pts_to a0 s0  `star` pts_to a1 s0)
+      (pts_to a0 p0 s0 `star` pts_to a1 full_perm s1)
+      (fun _ -> pts_to a0 p0 s0  `star` pts_to a1 full_perm s0)
   = let _ = elim_pts_to a0 s0 in
     let _ = elim_pts_to a1 s1 in
     A.elim_varray_pts_to a0 _;
@@ -185,21 +189,23 @@ let memcpy_pt (#t:_)
     return ()
 
 let memcpy (#t:_)
+           (#p0:perm)
            (a0 a1:array t)
            (#s0 #s1:erased (seq t))
            (l:U32.t { U32.v l == length a0 /\ length a0 == length a1 } )
   : STT unit
-    (pts_to a0 s0 `star` pts_to a1 s1)
-    (fun _ -> pts_to a0 s0  `star` pts_to a1 s0)
+    (pts_to a0 p0 s0 `star` pts_to a1 full_perm s1)
+    (fun _ -> pts_to a0 p0 s0  `star` pts_to a1 full_perm s0)
   = coerce_steel (fun _ -> memcpy_pt a0 a1 l); ()
 
 let compare_pt (#t:eqtype)
+               (#p0 #p1:perm)
                (a0 a1:array t)
                (#s0 #s1:erased (seq t))
                (l:U32.t { U32.v l == length a0 /\ length a0 == length a1 } )
   : SE.Steel bool
-    (pts_to a0 s0 `star` pts_to a1 s1)
-    (fun _ -> pts_to a0 s0 `star` pts_to a1 s1)
+    (pts_to a0 p0 s0 `star` pts_to a1 p1 s1)
+    (fun _ -> pts_to a0 p0 s0 `star` pts_to a1 p1 s1)
     (requires fun _ -> True)
     (ensures fun _ b _ -> b <==> eq2 #(Seq.seq t) s0 s1)
   = let _ = elim_pts_to a0 _ in
@@ -214,12 +220,13 @@ let compare_pt (#t:eqtype)
     return b
 
 let compare (#t:eqtype)
+            (#p0 #p1:perm)
             (a0 a1:array t)
             (#s0 #s1:erased (seq t))
             (l:U32.t { U32.v l == length a0 /\ length a0 == length a1 } )
   : ST bool
-    (pts_to a0 s0 `star` pts_to a1 s1)
-    (fun _ -> pts_to a0 s0 `star` pts_to a1 s1)
+    (pts_to a0 p0 s0 `star` pts_to a1 p1 s1)
+    (fun _ -> pts_to a0 p0 s0 `star` pts_to a1 p1 s1)
     (requires True)
     (ensures fun b -> b <==> eq2 #(Seq.seq t) s0 s1)
   = let b = coerce_steel (fun _ -> compare_pt a0 a1 l) in
